finish level two simplification (rewriting system version)

theories/LevelTwoSimp.v
@@ -5,14 +5,18 @@ Module O := LevelOne.
 Module T := LevelTwo.
 Import T.
 
-(** This file defines _irreducible_ forms for level two 
-    expressions/substitutions, i.e. expressions in which we can't
-    simplify anymore.
+(** This file defines a simplification algorithm for level two 
+    terms/substitutions. 
     
-    We first define _reducible_ forms (in which we can reduce),
-    and define irreducible as the negation of reducible.
+    We first define simplification as a rewriting system ([qred], [rred], 
+    [ered], [sred]), which is proved sound with respect to evaluation
+    (lemmas [ered_sound], [sred_sound], etc).
     
-    We then prove numerous lemmas that characterize irreducible forms. *)
+    We then implement simplification functions ([qsimp], [rsimp], [esimp], 
+    [ssimp]). We prove that the simplification functions indeed implement
+    the rewriting system (lemmas [qsimp_red], [rsimp_red], etc), and that 
+    they compute irreducible forms (lemmas [qsimp_irreducible], 
+    [rsimp_irreducible], etc). *)
 
 Section WithSignature.
 Context {sig : signature}.
@@ -77,8 +81,6 @@ Definition is_smvar_l s :=
 Definition is_sren_l s := 
   match s with S_comp (S_ren _) _ => true | _ => false end.
 
-
-
 (*********************************************************************************)
 (** *** Rewriting system. *)
 (*********************************************************************************)
@@ -134,9 +136,24 @@ Inductive ered : forall {k}, expr k -> expr k -> Prop :=
 | ered_congr_abind {ty} : Proper (ered ==> ered) (@E_abind _ ty)
 | ered_congr_ren {k} : Proper (rred ==> ered ==> ered) (@E_ren _ k)
 | ered_congr_subst {k} : Proper (sred ==> ered ==> ered) (@E_subst _ k)
-(* Simplification rules. *)
+(* Extract [Q_rapply] into [E_ren]. *)
 | ered_rapply r i : E_tvar (Q_rapply r i) =e=> E_ren r (E_tvar i)
-| ered_ren {k} r (t : expr k) : E_ren r t =e=> E_subst (S_ren r) t
+(* Simplify renamings. *)
+| ered_ren_ctor r c al : E_ren r (E_tctor c al) =e=> E_tctor c (E_ren r al)
+| ered_ren_al_nil r : E_ren r E_al_nil =e=> E_al_nil
+| ered_ren_al_cons {ty tys} r (a : expr (Ka ty)) (al : expr (Kal tys)) : 
+    E_ren r (E_al_cons a al) =e=> E_al_cons (E_ren r a) (E_ren r al)
+| ered_ren_abase r b x : E_ren r (E_abase b x) =e=> E_abase b x
+| ered_ren_aterm r t : E_ren r (E_aterm t) =e=> E_aterm (E_ren r t)
+| ered_ren_abind {ty} r (a : expr (Ka ty)) : 
+    E_ren r (E_abind a) =e=> E_abind (E_ren (R_cons Q_zero (R_comp r R_shift)) a)
+| ered_ren_ren {k} r1 r2 (t : expr k) : 
+    E_ren r2 (E_ren r1 t) =e=> E_ren (R_comp r1 r2) t
+| ered_ren_subst {k} r s (t : expr k) : 
+    E_ren r (E_subst s t) =e=> E_subst (S_comp s (S_ren r)) t
+| ered_ren_id {k} (t : expr k) : E_ren R_id t =e=> t
+| ered_ren_cons_zero i r : E_ren (R_cons i r) (E_tvar Q_zero) =e=> E_tvar i
+(* Simplify substitutions. *)
 | ered_subst_ctor s c al : E_subst s (E_tctor c al) =e=> E_tctor c (E_subst s al)
 | ered_subst_al_nil s : E_subst s E_al_nil =e=> E_al_nil
 | ered_subst_al_cons {ty tys} s (a : expr (Ka ty)) (al : expr (Kal tys)) : 
@@ -144,11 +161,14 @@ Inductive ered : forall {k}, expr k -> expr k -> Prop :=
 | ered_subst_abase s b x : E_subst s (E_abase b x) =e=> E_abase b x
 | ered_subst_aterm s t : E_subst s (E_aterm t) =e=> E_aterm (E_subst s t)
 | ered_subst_abind {ty} s (a : expr (Ka ty)) : 
-    E_subst s (E_abind a) =e=> E_abind (E_subst (S_cons (E_tvar Q_zero) (S_comp s S_shift)) a)
+    E_subst s (E_abind a) =e=> E_abind (E_subst (S_cons (E_tvar Q_zero) (S_comp s (S_ren R_shift))) a)
+| ered_subst_ren {k} s r (t : expr k) : 
+    E_subst s (E_ren r t) =e=> E_subst (S_comp (S_ren r) s) t
 | ered_subst_subst {k} s1 s2 (t : expr k) : 
     E_subst s2 (E_subst s1 t) =e=> E_subst (S_comp s1 s2) t
 | ered_subst_id {k} (t : expr k) : E_subst S_id t =e=> t
 | ered_subst_cons_zero t s : E_subst (S_cons t s) (E_tvar Q_zero) =e=> t
+| ered_subst_sren {k} r (t : expr k) : E_subst (S_ren r) t =e=> E_ren r t
 
 with sred : subst -> subst -> Prop :=
 (* Preorder. *)
@@ -243,10 +263,15 @@ apply ered_sred_ind ; intros ; simp eeval qeval ; triv.
 all: try solve [ now rewrite H0, H2 ]. 
 - eapply qred_sound in H. now rewrite H.
 - eapply rred_sound in H. now rewrite H1, H.
-- now rewrite O.ren_is_subst.
+- now rewrite O.ren_ren.
+- rewrite O.ren_subst. apply O.substitute_proper ; triv.
+  intros i. cbv [O.srcomp O.scomp]. now rewrite O.ren_is_subst.
+- now rewrite O.ren_rid. 
 - simp substitute. rewrite O.up_subst_alt. reflexivity.
+- rewrite O.subst_ren. apply O.substitute_proper ; triv.
 - now rewrite O.subst_subst.
 - now rewrite O.subst_sid.
+- now rewrite O.ren_is_subst.   
 - eapply rred_sound in H. now rewrite H.
 - now rewrite O.scomp_sid_r.
 - now rewrite O.scomp_assoc.
@@ -265,18 +290,18 @@ Proof. now apply ered_sred_sound. Qed.
 (** *** Irreducible & reducible forms. *)
 (*********************************************************************************)
 
-(** The "true" definition of irreducible forms, i.e. terms in which we can't 
-    reduce. This definition is obviously correct but is hard to work with. *)
-Definition qirred i := forall i', i =q=> i' -> i = i'.
-Definition rirred r := forall r', r =r=> r' -> r = r'.
-Definition eirred {k} (t : expr k) := forall t', t =e=> t' -> t = t'.
-Definition sirred s := forall s', s =s=> s' -> s = s'.
+(** The "true" definition of irreducible forms (terms in which we can't 
+    reduce). This definition is obviously correct but is hard to work with. *)
+Definition qirreducible i := forall i', i =q=> i' -> i = i'.
+Definition rirreducible r := forall r', r =r=> r' -> r = r'.
+Definition eirreducible {k} (t : expr k) := forall t', t =e=> t' -> t = t'.
+Definition sirreducible s := forall s', s =s=> s' -> s = s'.
 
 Unset Elimination Schemes.
 
-(** A definition of reducible forms, i.e. terms in which we can reduce,
+(** A definition of reducible forms (terms in which we can reduce)
     which is easy to work with but is not obviously correct.
-    We prove below that this notion agrees with [qirred], [rirred], etc. *)
+    We prove below that this notion agrees with [qirreducible], [rirreducible], etc. *)
 Inductive qreducible : qnat -> Prop :=
 (* Congruence. *)
 | qreducible_congr_succ i : qreducible i -> qreducible (Q_succ i)
@@ -303,8 +328,8 @@ with rreducible : ren -> Prop :=
 | rreducible_zero_shift : rreducible (R_cons Q_zero R_shift).
 
 (** Expressions in which we can push substitutions. *)
-Definition is_push {k} (e : expr k) : Prop :=
-  match e with E_mvar _ | E_tvar _ | E_ren _ _ => False | _ => True end.
+Definition is_push {k} (e : expr k) : bool :=
+  match e with E_mvar _ | E_tvar _ => false | _ => true end.
 
 Inductive ereducible : forall {k}, expr k -> Prop :=
 (* Congruence. *)
@@ -322,10 +347,13 @@ Inductive ereducible : forall {k}, expr k -> Prop :=
 | ereducible_congr_subst_2 {k} s (t : expr k) : ereducible t -> ereducible (E_subst s t)
 (* Simplification rules. *)
 | ereducible_rapply r i : ereducible (E_tvar (Q_rapply r i))
-| ereducible_ren {k} r (e : expr k) : ereducible (E_ren r e)
+| ereducible_ren {k} r (e : expr k) : is_push e -> ereducible (E_ren r e)
+| ereducible_ren_id {k} (e : expr k) : ereducible (E_ren R_id e)
+| ereducible_ren_cons_zero r : is_rcons r -> ereducible (E_ren r (E_tvar Q_zero))
 | ereducible_subst {k} s (e : expr k) : is_push e -> ereducible (E_subst s e)
 | ereducible_subst_id {k} (e : expr k) : ereducible (E_subst S_id e)
 | ereducible_subst_cons_zero s : is_scons s -> ereducible (E_subst s (E_tvar Q_zero))
+| ereducible_subst_sren {k} s (e : expr k) : is_sren s -> ereducible (E_subst s e)
 
 with sreducible : subst -> Prop :=
 (* Congruence. *)
@@ -361,6 +389,17 @@ Derive Signature for qreducible rreducible ereducible sreducible.
 (** *** Equivalence between the two notions of irreducible forms. *)
 (*********************************************************************************)
 
+(** [inv_subterm H] checks if [H] is an equality between 
+    expressions/substitutions/etc where one side is a subterm of the other,
+    and if so it solves the goal. *)
+Ltac inv_subterm H :=
+  lazymatch type of H with 
+  | @eq qnat _ _ => apply (f_equal qsize) in H ; simp qsize in H ; lia
+  | @eq ren _ _ => apply (f_equal rsize) in H ; simp qsize in H ; lia
+  | @eq (expr _) _ _ => apply (f_equal esize) in H ; simp esize in H ; lia
+  | @eq subst _ _ => apply (f_equal ssize) in H ; simp esize in H ; lia
+  end. 
+
 Lemma qr_red_impl_reducible : 
   (forall i i', i =q=> i' -> i = i' \/ qreducible i) /\ 
   (forall r r', r =r=> r' -> r = r' \/ rreducible r).
@@ -376,20 +415,18 @@ Proof.
 apply qreducible_rreducible_ind ; intros.
 all: try solve [ destruct H0 as (i' & H1 & H2) ; eexists ; split ; 
   [now rewrite H1 | intros H3 ; now depelim H3] ].
-- exists i. split ; triv. intros H. admit.
-  (*remember R_id as r. clear Heqr. 
-  induction i in r, H |- * ; triv. depelim H. symmetry in H. triv.*)
+- exists i. split ; triv. intros H ; inv_subterm H.
 - exists (Q_rapply (R_comp r2 r1) i). split ; triv. intros H ; depelim H.
-  admit.
-- destruct r ; triv. exists q. split ; triv. intros H1. admit.
+  inv_subterm H.
+- destruct r ; triv. exists q. split ; triv. intros H1. inv_subterm H1.
 - exists (Q_rapply R_shift i). split ; triv.
-- exists r. split ; triv. intros H. admit.
-- exists r. split ; triv. intros H. admit.
-- exists (R_comp r1 (R_comp r2 r3)). split ; triv. intros H. depelim H. admit.
+- exists r. split ; triv. intros H. inv_subterm H.
+- exists r. split ; triv. intros H. inv_subterm H.
+- exists (R_comp r1 (R_comp r2 r3)). split ; triv. intros H. depelim H. inv_subterm H.
 - exists (R_cons (Q_rapply r2 i) (R_comp r1 r2)). split ; triv.
-- destruct r ; triv. exists r. split ; triv. intros H1. admit.
+- destruct r ; triv. exists r. split ; triv. intros H1. inv_subterm H1.
 - exists R_id. split ; triv.
-Admitted.
+Qed.
 
 Lemma es_red_impl_reducible : 
   (forall {k} (t t' : expr k), t =e=> t' -> t = t' \/ ereducible t) /\ 
@@ -400,6 +437,8 @@ all: try solve [ destruct H0 ; triv | destruct H0, H2 ; triv ].
 all: try solve [ right ; apply ereducible_subst ; triv ]. 
 all: try solve [ right ; apply sreducible_sren ; triv ]. 
 - apply qr_red_impl_reducible in H. destruct H ; triv.
+- apply qr_red_impl_reducible in H. destruct H ; triv. subst.
+  destruct H1 ; triv.
 - apply qr_red_impl_reducible in H. destruct H ; triv.
 Qed.
 
@@ -414,52 +453,50 @@ all: try solve [ apply qr_reducible_impl_red in H ; destruct H as (i' & H1 & H2)
   eexists ; split ; [now rewrite H1 | intros H3 ; now depelim H3] ].
 - destruct H0 as (i' & H1 & H2). eexists. split ; [now rewrite H1 | intros H3]. admit.
 - exists (E_ren r (E_tvar i)). triv.
-- exists (E_subst (S_ren r) e). triv.
-- destruct e ; auto. 
-  + exists (E_tctor c (E_subst s e)). triv.
-  + exists E_al_nil. triv.
-  + exists (E_al_cons (E_subst s e1) (E_subst s e2)). triv.
-  + exists (E_abase b e). triv.
-  + exists (E_aterm (E_subst s e)). triv.
-  + eexists (E_abind (E_subst _ e)). triv.
-  + exists (E_subst (S_comp s0 s) e). split ; triv. intros H1. depelim H1. admit. 
-- exists e. split ; triv. admit.
-- destruct s ; triv. exists e. split ; triv. admit.  
-- exists s. split ; triv. admit.
-- exists s. split ; triv. admit.
-- exists (S_comp s1 (S_comp s2 s3)). split ; triv. admit.
+- destruct e ; try solve [ eexists ; triv ]. Unshelve. all: triv.
+  exists (E_ren (R_comp r0 r) e). split ; triv. intros H1. depelim H1. inv_subterm H0.
+- exists e. split ; triv. intros H. inv_subterm H. 
+- destruct r ; triv. exists (E_tvar q). split ; triv.
+- destruct e ; try solve [ eexists ; triv ]. Unshelve. all: triv.
+  + exists (E_subst (S_comp (S_ren r) s) e). split ; triv. intros H1. depelim H1.
+    inv_subterm H0.
+  + exists (E_subst (S_comp s0 s) e). split ; triv. intros H1. depelim H1. 
+    inv_subterm H0. 
+- exists e. split ; triv. intros H. inv_subterm H.
+- destruct s ; triv. exists e. split ; triv. intros H1. inv_subterm H1.
+- destruct s ; triv. exists (E_ren r e). split ; triv.
+- exists s. split ; triv. intros H. inv_subterm H. 
+- exists s. split ; triv. intros H. inv_subterm H. 
+- exists (S_comp s1 (S_comp s2 s3)). split ; triv. intros H. 
+  depelim H. inv_subterm H.
 - exists (S_cons (E_subst s2 t) (S_comp s1 s2)). split ; triv.
-- destruct s ; triv. exists s. split ; triv. admit.
+- destruct s ; triv. exists s. split ; triv. intros H1. inv_subterm H1.
 - exists S_id. triv.
-- destruct r ; auto.
-  + exists S_id. triv.
-  + exists S_shift. triv.
-  + eexists (S_cons _ _). triv.
-  + eexists (S_comp _ _). triv.     
+- destruct r ; eexists ; triv.
 Admitted.
 
-Lemma qirred_qreducible i : qirred i <-> ~qreducible i.
+Lemma qirreducible_qreducible i : qirreducible i <-> ~qreducible i.
 Proof.
 split.
 - intros H H'. apply qr_reducible_impl_red in H'. destruct H' as (i' & H1 & H2). triv.
 - intros H i' Hi. apply qr_red_impl_reducible in Hi. destruct Hi ; triv.
 Qed.
 
-Lemma rirred_rreducible r : rirred r <-> ~rreducible r.
+Lemma rirreducible_rreducible r : rirreducible r <-> ~rreducible r.
 Proof.
 split.
 - intros H H'. apply qr_reducible_impl_red in H'. destruct H' as (r' & H1 & H2). triv.
 - intros H r' Hr. apply qr_red_impl_reducible in Hr. destruct Hr ; triv.
 Qed.
 
-Lemma eirred_ereducible {k} (t : expr k) : eirred t <-> ~ereducible t.
+Lemma eirreducible_ereducible {k} (t : expr k) : eirreducible t <-> ~ereducible t.
 Proof.
 split.
 - intros H H'. apply es_reducible_impl_red in H'. destruct H' as (t' & H1 & H2). triv.
 - intros H t' Ht. apply es_red_impl_reducible in Ht. destruct Ht ; triv.
 Qed.
 
-Lemma sirred_sreducible s : sirred s <-> ~sreducible s.
+Lemma sirreducible_sreducible s : sirreducible s <-> ~sreducible s.
 Proof.
 split.
 - intros H H'. apply es_reducible_impl_red in H'. destruct H' as (s' & H1 & H2). triv.
@@ -467,24 +504,26 @@ split.
 Qed.
 
 Ltac change_irred :=
-  (repeat rewrite qirred_qreducible) ;
-  (repeat rewrite rirred_rreducible) ;
-  (repeat rewrite eirred_ereducible) ;
-  (repeat rewrite sirred_sreducible).
+  (repeat rewrite qirreducible_qreducible in *) ;
+  (repeat rewrite rirreducible_rreducible in *) ;
+  (repeat rewrite eirreducible_ereducible in *) ;
+  (repeat rewrite sirreducible_sreducible in *).
 
 (*********************************************************************************)
 (** *** Characterization of irreducible forms. *)
 (*********************************************************************************)
 
-Lemma qirred_zero : qirred Q_zero.
-Proof. change_irred. intros H. depelim H. Qed.
+Lemma qirreducible_zero : qirreducible Q_zero.
+Proof. change_irred. triv. Qed.
+#[local] Hint Resolve qirreducible_zero : core.
 
-Lemma qirred_succ i : ~qirred (Q_succ i).
+Lemma qirreducible_succ i : ~qirreducible (Q_succ i).
 Proof. change_irred. intros H. apply H. now constructor. Qed.
-    
-Lemma qirred_rapply r i : 
-  qirred (Q_rapply r i) <-> 
-    rirred r /\ qirred i /\ r <> R_id /\ ~is_qrapply i /\
+#[local] Hint Resolve qirreducible_succ : core.
+  
+Lemma qirreducible_rapply r i : 
+  qirreducible (Q_rapply r i) <-> 
+    rirreducible r /\ qirreducible i /\ r <> R_id /\ ~is_qrapply i /\
     ~(is_rcons r /\ i = Q_zero).
 Proof. 
 change_irred. split ; intros H. 
@@ -496,215 +535,885 @@ change_irred. split ; intros H.
   + destruct r ; triv. destruct H as (_ & _ & _ & _ & H). triv.
 Qed.
 
-Lemma qirred_mvar m : qirred (Q_mvar m).
+Lemma qirreducible_mvar m : qirreducible (Q_mvar m).
 Proof. change_irred. intros H. depelim H. Qed.
+#[local] Hint Resolve qirreducible_mvar : core.
 
-Lemma rirred_cons i r : 
-  rirred (R_cons i r) <-> 
-    qirred i /\ rirred r /\ ~(i = Q_zero /\ r = R_shift).
+Lemma rirreducible_id : rirreducible R_id.
+Proof. change_irred. triv. Qed.
+#[local] Hint Resolve rirreducible_id : core.
+
+Lemma rirreducible_shift : rirreducible R_shift.
+Proof. change_irred. triv. Qed.
+#[local] Hint Resolve rirreducible_shift : core.
+
+Lemma rirreducible_cons i r : 
+  rirreducible (R_cons i r) <-> 
+    qirreducible i /\ rirreducible r /\ ~(i = Q_zero /\ r = R_shift).
 Proof.
 change_irred. split.
 - intros H. split3 ; intros H' ; apply H ; triv.
   destruct H' ; subst. now constructor. 
-- intros (H1 & H2 & H3) H. depelim H.
-  + destruct H ; triv. apply H3 ; triv.
+- intros (H1 & H2 & H3) H. depelim H ; triv.
 Qed.
 
-Lemma rirred_mvar_l m r : 
-  rirred (R_comp (R_mvar m) r) <-> rirred r /\ r <> R_id.
-Proof.
-split.
-- intros H. split.
-  + intros H'. apply H ; clear H. apply RR_congr_comp. now right.
-  + intros H' ; subst. apply H. now constructor. 
-- intros (H & H') H''. depelim H'' ; triv. now destruct H0.
-Qed.      
-
-Lemma rirred_shift_l r : 
-  rirred (R_comp R_shift r) <-> 
-    rirred r /\ r <> R_id /\ ~is_rcons r.
-Proof.
-split.
-- intros H. split3 ; triv. intros H' ; apply H ; triv.
-- intros (H1 & H2 & H3) H. depelim H ; triv. destruct H ; triv.
-Qed.
-
-Lemma rirred_comp r1 r2 : 
-  rirred (R_comp r1 r2) <->
-    rirred r1 /\ rirred r2 /\ ~is_rcomp r1 /\ ~is_rcons r1 /\ 
+Lemma rirreducible_comp r1 r2 : 
+  rirreducible (R_comp r1 r2) <->
+    rirreducible r1 /\ rirreducible r2 /\ ~is_rcomp r1 /\ ~is_rcons r1 /\ 
     r1 <> R_id /\ r2 <> R_id /\ ~(r1 = R_shift /\ is_rcons r2).
 Proof.
-split ; intros H.
+change_irred. split ; intros H.
 - split7 ; intros H' ; apply H ; triv.
   + destruct r1 ; triv.
   + destruct r1 ; triv.
   + destruct H' as [-> H']. destruct r2 ; triv.
 - intros H' ; depelim H' ; triv.
-  + destruct H0 ; triv.
   + destruct H as (_ & _ & H & _) ; triv.
   + destruct H as (_ & _ & _ & H & _) ; triv.
   + destruct r2 ; triv. destruct H as (_ & _ & _ & _ & _ & _ & H). triv.
 Qed. 
 
-(*********************************************************************************)
-(** *** Irreducible forms for substitutions & expressions. *)
-(*********************************************************************************)
+Lemma rirreducible_mvar m : rirreducible (R_mvar m).
+Proof. change_irred. intros H. depelim H. Qed.
+#[local] Hint Resolve rirreducible_mvar : core.
 
-(** Reducible expression. *)
-Inductive ered : forall {k}, expr k -> Prop :=
-
-(** Congruence. *)
-| ER_congr_tvar i : qred i -> ered (E_tvar i)
-| ER_congr_tctor c al : ered al -> ered (E_tctor c al)
-| ER_congr_al_cons {ty} {tys} (a : arg ty) (al : args tys) : ered a \/ ered al -> ered (E_al_cons a al)
-| ER_congr_aterm t : ered t -> ered (E_aterm t)
-| ER_congr_abind {ty} (a : arg ty) : ered a -> ered (E_abind a) 
-| ER_congr_ren {k} r (e : expr k) : rred r \/ ered e -> ered (E_ren r e)
-| ER_congr_subst {k} s (e : expr k) : sred s \/ ered e -> ered (E_subst s e)
-
-(** Reduce [E_tvar (r i)] into [(E_tvar i)[S_ren r]]. *)
-| ER_extract_rapply r i : ered (E_tvar (Q_rapply r i))
-(** Reduce [rename r e] into [substitute (S_ren r) e]. *)
-| ER_extract_ren {k} r (e : expr k) : ered (E_ren r e)
-(** Push substitutions inside expressions. *)
-| ER_push_subst {k} s (e : expr k) : is_push e -> ered (E_subst s e)
-(** Reduce [e[sid]] into [e]. *)
-| ER_subst_sid {k} (e : expr k) : ered (E_subst S_id e)
-(** Reduce [0[t . s]] into [t]. *)
-| ER_scons_zero s : is_scons s -> ered (E_subst s (E_tvar Q_zero))
-
-(** Reducible substitutions. *)
-with sred : subst -> Prop :=
-
-(** Congruence. *)
-| SR_cons t s : ered t \/ sred s -> sred (S_cons t s)
-| SR_comp s1 s2 : sred s1 \/ sred s2 -> sred (S_comp s1 s2)
-| SR_ren r : rred r -> sred (S_ren r)
-
-(** Reduce [sid >> s] into [s]. *)
-| SR_sid_l s : sred (S_comp S_id s)
-(** Reduce [s >> sid] into [s]. *)
-| SR_sid_r s : sred (S_comp s S_id)
-(** Reduce [(s1 >> s2) >> s3] into [s1 >> (s2 >> s3)]. *)
-| SR_comp_l s1 s2 s3: sred (S_comp (S_comp s1 s2) s3)
-(** Push [S_ren] into renamings. *)
-| SR_ren_distrib r : ~is_rmvar r -> sred (S_ren r)
-(** Composition distributes over [S_cons]. *)
-| SR_cons_l t s1 s2 : sred (S_comp (S_cons t s1) s2)
-(** Reduce [shift >> (t . s)] into [s]. *)
-| SR_shift_cons s : is_scons s -> sred (S_comp S_shift s)
-(** Reduce [0 . shift] into [sid]. *)
-| SR_zero_shift : sred (S_cons (E_tvar Q_zero) S_shift)
-(** Reduce [s 0 . (shift >> s)] into [s]. *)
-(*| SR_zero_shift_l s : sred (S_cons (E_subst s (E_tvar Q_zero)) (S_comp S_shift s))*).
-
-Derive Signature for ered sred.
-
-Hint Constructors ered : core.
-Hint Constructors sred : core.
-
-(** Irreducible expressions/substitutions. *)
-Definition eirred {k} (e : expr k) := ~ered e.
-Definition sirred s := ~sred s.
-
-(*********************************************************************************)
-(** *** Characterization of irreducible forms for expressions & substitutions. *)
-(*********************************************************************************)
-
-Lemma eirred_tvar i : 
-  eirred (E_tvar i) <-> ~is_qrapply i /\ ~is_qsucc i.
+Lemma eirreducible_tvar i : 
+  eirreducible (E_tvar i) <-> ~is_qrapply i /\ ~is_qsucc i.
 Proof. 
-split ; intros H.
+change_irred. split ; intros H.
 - split ; intros H' ; apply H ; destruct i ; triv.
 - intros H'. destruct H. destruct i ; triv.
-  + depelim H'. depelim H1.
-  + depelim H'. depelim H1.
+  + depelim H' ; triv.
+  + depelim H' ; triv.
 Qed.
 
-Lemma eirred_tvar_zero : eirred (E_tvar Q_zero).
-Proof. intros H. depelim H. depelim H. Qed.
+Lemma eirreducible_tvar_zero : eirreducible (E_tvar Q_zero).
+Proof. change_irred. intros H. depelim H ; triv. Qed.
+#[local] Hint Resolve eirreducible_tvar_zero : core.
 
-Lemma eirred_mvar m : eirred (E_mvar m).
-Proof. intros H. depelim H. Qed.
+Lemma eirreducible_tctor c al : eirreducible (E_tctor c al) <-> eirreducible al.
+Proof. change_irred. split ; intros H H' ; apply H ; triv. now depelim H'. Qed.
 
-Lemma eirred_tctor c al : eirred (E_tctor c al) <-> eirred al.
-Proof. split ; intros H H' ; apply H ; triv. now depelim H'. Qed.
+Lemma eirreducible_al_nil : eirreducible E_al_nil.
+Proof. change_irred. intros H ; depelim H. Qed.
+#[local] Hint Resolve eirreducible_al_nil : core.
 
-Lemma eirred_al_nil : eirred E_al_nil.
-Proof. intros H ; depelim H. Qed.
-
-Lemma eirred_al_cons {ty tys} (a : arg ty) (al : args tys) :
-  eirred (E_al_cons a al) <-> eirred a /\ eirred al.
+Lemma eirreducible_al_cons {ty tys} (a : expr (Ka ty)) (al : expr (Kal tys)) :
+  eirreducible (E_al_cons a al) <-> eirreducible a /\ eirreducible al.
 Proof.
-split ; intros H.
+change_irred. split ; intros H.
 - split ; intros H' ; apply H ; triv.
-- intros H' ; depelim H' ; triv. destruct H0 ; triv.
+- intros H' ; depelim H' ; triv.
 Qed.
 
-Lemma eirred_abase b x : eirred (E_abase b x).
-Proof. triv. Qed.
+Lemma eirreducible_abase b x : eirreducible (E_abase b x).
+Proof. change_irred. triv. Qed.
+#[local] Hint Resolve eirreducible_abase : core.
 
-Lemma eirred_aterm t : eirred (E_aterm t) <-> eirred t.
-Proof. split ; intros H H' ; apply H ; triv. now depelim H'. Qed.
+Lemma eirreducible_aterm t : eirreducible (E_aterm t) <-> eirreducible t.
+Proof. change_irred. split ; intros H H' ; apply H ; triv. now depelim H'. Qed.
 
-Lemma eirred_abind {ty} (a : arg ty) : 
-  eirred (E_abind a) <-> eirred a.
-Proof. split ; intros H H' ; apply H ; triv. now depelim H'. Qed.
+Lemma eirreducible_abind {ty} (a : expr (Ka ty)) : 
+  eirreducible (E_abind a) <-> eirreducible a.
+Proof. change_irred. split ; intros H H' ; apply H ; triv. now depelim H'. Qed.
 
-Lemma eirred_ren {k} (e : expr k) r : ~eirred (E_ren r e).
-Proof. intros H ; apply H. triv. Qed.
-
-Lemma eirred_subst {k} (e : expr k) s :
-  eirred (E_subst s e) <->
-    eirred e /\ sirred s /\ ~is_push e /\
-    ~(is_tvar_zero e /\ is_scons s) /\ s <> S_id.
-Proof.
-split ; intros H.
+Lemma eirreducible_ren {k} (e : expr k) r :
+  eirreducible (E_ren r e) <-> 
+    rirreducible r /\ eirreducible e /\ ~is_push e /\
+    ~(is_rcons r /\ is_tvar_zero e) /\ r <> R_id.
+Proof. 
+change_irred. split ; intros H.
 - split5 ; intros H' ; apply H ; triv.
+  destruct e ; triv. destruct q ; triv. destruct r ; triv.
+- intros H' ; depelim H' ; triv.
+  destruct r ; triv. destruct H as (_ & _ & _ & H & _). triv.
+Qed.
+
+Lemma eirreducible_subst {k} (e : expr k) s :
+  eirreducible (E_subst s e) <->
+    eirreducible e /\ sirreducible s /\ ~is_push e /\
+    ~(is_tvar_zero e /\ is_scons s) /\ s <> S_id /\ ~is_sren s.
+Proof.
+change_irred. split ; intros H.
+- split6 ; intros H' ; apply H ; triv.
   destruct e ; triv. destruct q ; triv. destruct s ; triv.
 - intros H' ; depelim H' ; triv.
-  + destruct H0 ; triv.
-  + destruct s ; triv.
-    destruct H as (_ & _ & _ & H & _). triv.
+  destruct s ; triv. destruct H as (_ & _ & _ & H & _). triv.
 Qed.     
 
-Lemma sirred_mvar m : sirred (S_mvar m).
-Proof. intros H. depelim H. Qed.
+Lemma eirreducible_mvar m : eirreducible (E_mvar m).
+Proof. change_irred. triv. Qed.
+#[local] Hint Resolve eirreducible_mvar : core.
 
-Lemma sirred_cons t s : 
-  sirred (S_cons t s) <-> 
-    eirred t /\ sirred s /\ ~(t = E_tvar Q_zero /\ s = S_shift).
+Lemma sirreducible_id : sirreducible S_id.
+Proof. change_irred. triv. Qed.
+#[local] Hint Resolve sirreducible_id : core.
+
+Lemma sirreducible_shift : sirreducible S_shift.
+Proof. change_irred. triv. Qed.
+#[local] Hint Resolve sirreducible_shift : core.
+
+Lemma sirreducible_cons t s : 
+  sirreducible (S_cons t s) <-> 
+    eirreducible t /\ sirreducible s /\ ~(t = E_tvar Q_zero /\ s = S_shift).
 Proof.
-split ; intros H.
-- split3 ; intros H' ; apply H ; clear H.
-  + constructor ; now left.
-  + constructor ; now right.
-  + destruct H' ; subst. now constructor. 
-- intros H'. depelim H'. destruct H0 ; triv. destruct H as (_ & _ & H). triv.
+change_irred. split ; intros H.
+- split3 ; intros H' ; apply H ; triv.
+  destruct H' ; subst. now constructor. 
+- intros H'. depelim H' ; triv. destruct H as (_ & _ & H). triv.
 Qed.   
 
-Lemma sirred_ren r : sirred (S_ren r) <-> is_rmvar r.
-Proof.
-split ; intros H.
-- destruct r ; triv. all: exfalso ; apply H ; now constructor.
-- intros H' ; depelim H' ; triv. destruct r ; triv.
-Qed.
-
-Lemma sirred_comp s1 s2 : 
-  sirred (S_comp s1 s2) <->
-    sirred s1 /\ sirred s2 /\ ~is_scomp s1 /\ ~is_scons s1 /\ 
+Lemma sirreducible_comp s1 s2 : 
+  sirreducible (S_comp s1 s2) <->
+    sirreducible s1 /\ sirreducible s2 /\ ~is_scomp s1 /\ ~is_scons s1 /\ 
     s1 <> S_id /\ s2 <> S_id /\ ~(s1 = S_shift /\ is_scons s2).
 Proof.
-split ; intros H.
+change_irred. split ; intros H.
 - split7 ; intros H' ; apply H ; triv.
   + destruct s1 ; triv.
   + destruct s1 ; triv.
   + destruct H' as [-> H']. destruct s2 ; triv.
 - intros H' ; depelim H' ; triv.
-  + destruct H0 ; triv.
   + destruct H as (_ & _ & H & _) ; triv.
   + destruct H as (_ & _ & _ & H & _) ; triv.
   + destruct s2 ; triv. destruct H as (_ & _ & _ & _ & _ & _ & H). triv.
 Qed. 
 
-End Make.
+Lemma sirreducible_ren r : sirreducible (S_ren r) <-> is_rmvar r.
+Proof.
+change_irred. split ; intros H.
+- destruct r ; triv. all: exfalso ; apply H ; now constructor.
+- intros H' ; depelim H' ; triv. destruct r ; triv.
+Qed.
+
+Lemma sirreducible_mvar m : sirreducible (S_mvar m).
+Proof. change_irred. intros H. depelim H. Qed.
+#[local] Hint Resolve sirreducible_mvar : core.
+
+(*********************************************************************************)
+(** *** [rapply_aux] *)
+(*********************************************************************************)
+
+(** Helper function for [rapply] which takes care of trivial cases. *)
+Equations rapply_aux (r : ren) (i : qnat) : qnat :=
+rapply_aux R_id i := i ;
+rapply_aux (R_cons k r) Q_zero := k ;
+rapply_aux r i := Q_rapply r i.
+
+Lemma rapply_aux_red r i : Q_rapply r i =q=> rapply_aux r i.
+Proof. funelim (rapply_aux r i) ; triv. Qed.
+#[local] Hint Rewrite <-rapply_aux_red : red.
+
+Lemma rapply_aux_irreducible r i : 
+  rirreducible r -> qirreducible i -> 
+  (r <> R_id -> ~(is_rcons r /\ i = Q_zero) -> qirreducible (Q_rapply r i)) -> 
+  qirreducible (rapply_aux r i).
+Proof.
+intros H1 H2 H3. funelim (rapply_aux r i) ; triv.
+all: try solve [ apply H3 ; triv ].
+rewrite rirreducible_cons in H1 ; triv.
+Qed.   
+
+(*********************************************************************************)
+(** *** [rcomp_aux] *)
+(*********************************************************************************)
+
+(** Helper function for [rcomp] which takes care of trivial cases. *)
+Equations rcomp_aux (r1 r2 : ren) : ren :=
+rcomp_aux r R_id := r ;
+rcomp_aux R_shift (R_cons _ r) := r ;
+rcomp_aux r1 r2 := R_comp r1 r2.
+
+Lemma rcomp_aux_red r1 r2 : R_comp r1 r2 =r=> rcomp_aux r1 r2.
+Proof. funelim (rcomp_aux r1 r2) ; triv. Qed.
+#[local] Hint Rewrite <-rcomp_aux_red : red.
+
+Lemma rcomp_aux_irreducible r1 r2 : 
+  rirreducible r1 -> rirreducible r2 -> 
+  (r2 <> R_id -> ~(r1 = R_shift /\ is_rcons r2) -> rirreducible (R_comp r1 r2)) -> 
+  rirreducible (rcomp_aux r1 r2).
+Proof.
+intros H1 H2 H3. funelim (rcomp_aux r1 r2) ; triv.
+all: try solve [ apply H3 ; now triv ].
+now rewrite rirreducible_cons in H2.
+Qed.
+
+(*********************************************************************************)
+(** *** [rcons] *)
+(*********************************************************************************)
+
+Equations rcons : qnat -> ren -> ren :=
+rcons Q_zero R_shift := R_id ;
+rcons i r := R_cons i r.
+
+Lemma rcons_red i r : R_cons i r =r=> rcons i r.
+Proof. funelim (rcons i r) ; triv. Qed.
+#[local] Hint Rewrite <-rcons_red : red.
+
+Lemma rcons_irreducible i r :
+  qirreducible i -> rirreducible r -> rirreducible (rcons i r).
+Proof.
+intros H1 H2. funelim (rcons i r) ; triv.
+all: solve [ rewrite rirreducible_cons ; triv ].
+Qed. 
+
+(*********************************************************************************)
+(** *** [rapply] and [rcomp] *)
+(*********************************************************************************)
+
+(** Simplify [Q_rapply r i]. *)
+Equations rapply (r : ren) (i : qnat) : qnat by struct i := 
+rapply r (Q_rapply r' i) := rapply_aux (rcomp r' r) i ;
+rapply r i := rapply_aux r i
+
+(** Simplify [R_comp r1 r2]. *)
+with rcomp (r1 r2 : ren) : ren by struct r1 :=
+rcomp R_id r := r ;
+rcomp (R_cons i r1) r2 := rcons (rapply r2 i) (rcomp r1 r2) ;
+rcomp (R_comp r1 r2) r3 := rcomp r1 (rcomp r2 r3) ;
+rcomp r1 r2 := rcomp_aux r1 r2.
+
+Lemma rapply_rcomp_red :
+  (forall r i, Q_rapply r i =q=> rapply r i) *
+  (forall r1 r2, R_comp r1 r2 =r=> rcomp r1 r2).
+Proof.
+apply rapply_elim with 
+  (P := fun r i res => Q_rapply r i =q=> res)
+  (P0 := fun r1 r2 res => R_comp r1 r2 =r=> res).
+all: intros ; simp red ; triv.
+- rewrite <-H. triv.
+- rewrite <-H, <-H0. triv. 
+- rewrite <-H0, <-H. triv. 
+Qed.
+
+Lemma rapply_red r i : Q_rapply r i =q=> rapply r i.
+Proof. now apply rapply_rcomp_red. Qed.
+#[local] Hint Rewrite <-rapply_red : red.
+
+Lemma rcomp_red r1 r2 : R_comp r1 r2 =r=> rcomp r1 r2.
+Proof. now apply rapply_rcomp_red. Qed.
+#[local] Hint Rewrite <-rcomp_red : red.
+
+Lemma rapply_rcomp_irreducible :
+  (forall r i, rirreducible r -> qirreducible i -> qirreducible (rapply r i)) *
+  (forall r1 r2, rirreducible r1 -> rirreducible r2 -> rirreducible (rcomp r1 r2)).
+Proof.
+apply rapply_elim with 
+  (P := fun r i res => rirreducible r -> qirreducible i -> qirreducible res)
+  (P0 := fun r1 r2 res => rirreducible r1 -> rirreducible r2 -> rirreducible res).
+all: intros ; triv.
+- apply rapply_aux_irreducible ; triv. intros H1 H2. rewrite qirreducible_rapply ; triv.
+- now apply qirreducible_succ in H0.
+- rewrite qirreducible_rapply in H1. apply rapply_aux_irreducible ; triv. 
+  + now apply H.
+  + intros H2 H3. rewrite qirreducible_rapply. split5 ; triv. now apply H.
+- apply rapply_aux_irreducible ; triv. intros H1 H2. rewrite qirreducible_rapply.
+  split5 ; triv.
+- apply rcomp_aux_irreducible ; triv. intros H1 H2. rewrite rirreducible_comp.
+  split3 ; triv.
+- rewrite rirreducible_cons in *. apply rcons_irreducible.
+  + now apply H.
+  + now apply H0.
+- rewrite rirreducible_comp in H1. apply H0 ; triv. apply H ; triv.
+- apply rcomp_aux_irreducible ; triv. intros H1 H2. rewrite rirreducible_comp. triv.
+Qed. 
+
+(*********************************************************************************)
+(** *** [qsimp] and [rsimp] *)
+(*********************************************************************************)
+
+(** Simplify a quoted natural. *)
+Equations qsimp : qnat -> qnat :=
+qsimp Q_zero := Q_zero ;
+qsimp (Q_succ i) := rapply R_shift (qsimp i) ;
+qsimp (Q_rapply r i) := rapply (rsimp r) (qsimp i) ;
+qsimp (Q_mvar m) := Q_mvar m 
+
+(** Simplify a renaming. *)
+with rsimp : ren -> ren :=
+rsimp (R_cons i r) := rcons (qsimp i) (rsimp r) ;
+rsimp (R_comp r1 r2) := rcomp (rsimp r1) (rsimp r2) ;
+rsimp r := r.
+
+Lemma qsimp_rsimp_red :
+  (forall i, i =q=> qsimp i) * (forall r, r =r=> rsimp r).
+Proof. 
+apply qsimp_elim with 
+  (P := fun i res => i =q=> res)
+  (P0 := fun r res => r =r=> res).
+all: intros ; simp red ; triv.
+- now rewrite <-H, <-H0.
+- now rewrite <-H, <-H0.
+- now rewrite <-H, <-H0. 
+Qed.    
+
+Lemma qsimp_red i : i =q=> qsimp i.
+Proof. now apply qsimp_rsimp_red. Qed.
+#[local] Hint Rewrite <-qsimp_red : red.
+
+Lemma rsimp_red r : r =r=> rsimp r.
+Proof. now apply qsimp_rsimp_red. Qed.
+#[local] Hint Rewrite <-rsimp_red : red.
+
+Lemma qsimp_rsimp_irreducible : 
+  (forall i, qirreducible (qsimp i)) * (forall r, rirreducible (rsimp r)).
+Proof.
+apply qsimp_elim with 
+  (P := fun _ res => qirreducible res) 
+  (P0 := fun _ res => rirreducible res).
+all: intros ; try solve [ change_irred ; triv ].
+- now apply rapply_rcomp_irreducible.
+- now apply rapply_rcomp_irreducible.
+- now apply rcons_irreducible.
+- now apply rapply_rcomp_irreducible.
+Qed.
+
+Lemma qsimp_irreducible i : qirreducible (qsimp i).
+Proof. now apply qsimp_rsimp_irreducible. Qed.
+
+Lemma rsimp_irreducible r : rirreducible (rsimp r).
+Proof. now apply qsimp_rsimp_irreducible. Qed.
+
+(*********************************************************************************)
+(** *** [scons] *)
+(*********************************************************************************)
+
+(** Simplify [S_cons t s].
+    We use a traditional pattern match instead of a [with] clause because 
+    we want to avoid using [NoConfusion] in the generated code. *)
+Equations scons (t : expr Kt) (s : subst) : subst :=
+scons t S_shift := match t with E_tvar Q_zero => S_id | _ => S_cons t S_shift end ;
+scons t s := S_cons t s. 
+
+Lemma scons_red t s : S_cons t s =s=> scons t s. 
+Proof.
+funelim (scons t s) ; triv. depelim t ; triv. depelim q ; triv.
+Qed.
+#[local] Hint Rewrite <-scons_red : red.
+
+Lemma scons_irreducible t s :
+  eirreducible t -> sirreducible s -> sirreducible (scons t s).
+Proof.
+intros H1 H2. 
+funelim (scons t s) ; try solve [ rewrite sirreducible_cons ; triv ].
+depelim t ; try solve [ rewrite sirreducible_cons ; triv ].
+depelim q ; try solve [ rewrite sirreducible_cons ; triv ]. triv.
+Qed. 
+
+(*********************************************************************************)
+(** *** [tnat] *)
+(*********************************************************************************)
+
+(** Simplify [E_tvar i]. We take care of extracting [Q_rapply] into [E_ren]. *)
+Equations tnat : qnat -> expr Kt :=
+tnat (Q_rapply r i) := E_ren r (E_tvar i) ; 
+tnat i := E_tvar i.
+
+Lemma tnat_red i : E_tvar i =e=> tnat i.
+Proof. funelim (tnat i) ; triv. Qed.
+#[local] Hint Rewrite <-tnat_red : red.
+
+Lemma tnat_irreducible i : qirreducible i -> eirreducible (tnat i).
+Proof.
+intros H. funelim (tnat i) ; triv.
+- now apply qirreducible_succ in H.
+- rewrite qirreducible_rapply in H. rewrite eirreducible_ren. split5 ; triv.
+  + rewrite eirreducible_tvar. split ; triv. destruct i ; triv. 
+    destruct H as (_ & H & _). now apply qirreducible_succ in H.
+  + intros (H1 & H2). destruct i ; triv. destruct r ; triv.
+    destruct H as (_ & _ & _ & _ & H). triv.
+- rewrite eirreducible_tvar. triv.
+Qed.
+
+(*********************************************************************************)
+(** *** [sren] *)
+(*********************************************************************************)
+
+(** Simplify [S_ren r]. *)
+Equations sren (r : ren) : subst :=
+sren R_id := S_id ;
+sren R_shift := S_shift ;
+sren (R_cons i r) := S_cons (tnat i) (sren r) ;
+sren (R_comp r1 r2) := S_comp (sren r1) (sren r2) ;
+sren (R_mvar r) := S_ren (R_mvar r).
+
+Lemma sren_red r : S_ren r =s=> sren r.
+Proof. 
+funelim (sren r) ; simp red ; triv.
+- rewrite <-H. triv.
+- rewrite <-H, <-H0. triv.
+Qed.  
+#[local] Hint Rewrite <-sren_red : red.
+
+Lemma sren_irreducible r :
+  rirreducible r -> sirreducible (sren r).
+Proof.
+intros H. funelim (sren r) ; triv.
+- rewrite rirreducible_cons in H0. rewrite sirreducible_cons. split3.
+  + now apply tnat_irreducible.
+  + now apply H.
+  + intros (H2 & H3). destruct H0 as (_ & _ & H0) ; apply H0. split.
+    * destruct i ; triv.
+    * destruct r ; triv.  
+- rewrite rirreducible_comp in H1. feed H ; triv. feed H0 ; triv.
+  rewrite sirreducible_comp. split7 ; triv.
+  + destruct r1 ; triv.
+  + destruct r1 ; triv.
+  + destruct r1 ; triv.
+  + destruct r2 ; triv.
+  + destruct r1 ; triv. destruct r2 ; triv.
+    destruct H1 as (_ & _ & _ & _ & _ & _ & H1). triv.     
+- rewrite sirreducible_ren. triv.
+Qed.
+
+(*********************************************************************************)
+(** *** [scomp_aux] *)
+(*********************************************************************************)
+
+(** Helper function for [rscomp], [srcomp], and [scomp]
+    which takes care of trivial cases. *)
+Equations scomp_aux : subst -> subst -> subst :=
+scomp_aux s S_id := s ;
+scomp_aux S_shift (S_cons t s) := s ;
+scomp_aux s1 s2 := S_comp s1 s2.
+
+Lemma scomp_aux_red s1 s2 : S_comp s1 s2 =s=> scomp_aux s1 s2. 
+Proof. funelim (scomp_aux s1 s2) ; triv. Qed.
+#[local] Hint Rewrite <-scomp_aux_red : red.
+
+Lemma scomp_aux_irreducible s1 s2 :
+  sirreducible s1 -> sirreducible s2 -> 
+  (s2 <> S_id -> ~(s1 = S_shift /\ is_scons s2) -> sirreducible (S_comp s1 s2)) ->
+  sirreducible (scomp_aux s1 s2).
+Proof.
+intros H1 H2 H3. funelim (scomp_aux s1 s2) ; triv.
+all: try solve [ apply H3 ; triv ]. 
+now rewrite sirreducible_cons in H2.
+Qed.
+
+(*********************************************************************************)
+(** *** [sapply_aux] *)
+(*********************************************************************************)
+
+(** Helper function for [sapply] which takes care of trivial cases. *)
+Equations sapply_aux : subst -> qnat -> expr Kt :=
+sapply_aux S_id i := E_tvar i ;
+sapply_aux (S_cons t _) Q_zero := t ;
+sapply_aux (S_ren r) i with i := {
+  | Q_rapply r' i' => E_ren (rcomp r' r) (E_tvar i')
+  | i' => E_ren r (E_tvar i')
+  } ;
+sapply_aux s i := E_subst s (E_tvar i).
+
+Lemma sapply_aux_red s i : E_subst s (E_tvar i) =e=> sapply_aux s i. 
+Proof. 
+funelim (sapply_aux s i) ; simp red ; triv.
+rewrite ered_subst_sren, ered_rapply. triv.
+Qed.
+#[local] Hint Rewrite <-sapply_aux_red : red.
+
+Lemma sapply_aux_irreducible s i :
+  sirreducible s -> qirreducible i -> ~is_qrapply i ->
+  (s <> S_id -> ~(is_scons s /\ i = Q_zero) -> ~is_sren s -> eirreducible (E_subst s (E_tvar i))) ->
+  eirreducible (sapply_aux s i).
+Proof.
+intros H1 H2 H3 H4. funelim (sapply_aux s i).
+all: try solve [ apply H4 ; triv ].
+- rewrite eirreducible_tvar. destruct i ; triv. now apply qirreducible_succ in H2.  
+- now rewrite sirreducible_cons in H1.
+- rewrite sirreducible_ren in H1. destruct r ; triv. rewrite eirreducible_ren. triv.
+- now apply qirreducible_succ in H2.
+- exfalso. triv.
+- rewrite sirreducible_ren in H1. destruct r ; triv. rewrite eirreducible_ren. 
+  split5 ; triv. rewrite eirreducible_tvar. triv.
+Qed.
+
+(*********************************************************************************)
+(** *** [sapply] and [rscomp] *)
+(*********************************************************************************)
+
+(** Simplify [E_subst s (E_tvar i)]. *)
+Equations sapply (s : subst) (i : qnat) : expr Kt by struct i :=
+sapply s (Q_rapply r i) := sapply_aux (rscomp r s) i ;
+sapply s i := sapply_aux s i
+
+(** Simplify [S_comp (S_ren r) s]. *)
+with rscomp (r : ren) (s : subst) : subst by struct r :=
+rscomp R_id s := s ;
+rscomp R_shift s := scomp_aux S_shift s ;
+rscomp (R_cons i r) s := scons (sapply s i) (rscomp r s) ;
+rscomp (R_comp r1 r2) s := rscomp r1 (rscomp r2 s) ;
+rscomp (R_mvar m) s := scomp_aux (S_ren (R_mvar m)) s.
+
+Lemma sapply_rscomp_red :
+  (forall s i, E_subst s (E_tvar i) =e=> sapply s i) *
+  (forall r s, S_comp (S_ren r) s =s=> rscomp r s).
+Proof.
+apply sapply_elim with 
+  (P := fun s i res => E_subst s (E_tvar i) =e=> res)
+  (P0 := fun r s res => S_comp (S_ren r) s =s=> res).
+all: intros ; simp red ; triv.
+- rewrite <-H. rewrite ered_rapply. triv.
+- rewrite sred_sren_id. triv.
+- rewrite sred_sren_shift. triv.
+- rewrite <-H, <-H0. rewrite sred_sren_cons. triv.
+- rewrite <-H0, <-H. rewrite sred_sren_comp. triv.  
+Qed. 
+
+Lemma sapply_red s i : E_subst s (E_tvar i) =e=> sapply s i.
+Proof. now apply sapply_rscomp_red. Qed.
+#[local] Hint Rewrite <-sapply_red : red.
+
+Lemma rscomp_red r s : S_comp (S_ren r) s =s=> rscomp r s.
+Proof. now apply sapply_rscomp_red. Qed.
+#[local] Hint Rewrite <-rscomp_red : red.
+
+Lemma sapply_rscomp_irreducible :
+  (forall s i, sirreducible s -> qirreducible i -> eirreducible (sapply s i)) *
+  (forall r s, rirreducible r -> sirreducible s -> sirreducible (rscomp r s)).
+Proof.
+apply sapply_elim with 
+  (P := fun s i res => sirreducible s -> qirreducible i -> eirreducible res)
+  (P0 := fun r s res => rirreducible r -> sirreducible s -> sirreducible res).
+all: intros ; triv.
+- apply sapply_aux_irreducible ; triv. intros H1 H2. rewrite eirreducible_subst.
+  split5 ; triv. intros [? ?] ; triv.
+- now apply qirreducible_succ in H0.
+- rewrite qirreducible_rapply in H1. apply sapply_aux_irreducible ; triv. 
+  + now apply H.
+  + intros H2 H3. rewrite eirreducible_subst. split5 ; triv.
+    * rewrite eirreducible_tvar. destruct i ; triv. destruct H1 as (_ & H1 & _).
+      now apply qirreducible_succ in H1.
+    * now apply H.
+    * intros [? ?] ; destruct i ; triv.
+- apply sapply_aux_irreducible ; triv.   intros H1 H2. rewrite eirreducible_subst.
+  split5 ; triv. rewrite eirreducible_tvar ; triv. 
+- apply scomp_aux_irreducible ; triv. intros H1. rewrite sirreducible_comp. triv. 
+- rewrite rirreducible_cons in H1. apply scons_irreducible. 
+  + apply H ; triv.
+  + apply H0 ; triv.
+- rewrite rirreducible_comp in H1. apply H0 ; triv. apply H ; triv.
+- apply scomp_aux_irreducible ; triv.
+  + rewrite sirreducible_ren ; triv.
+  + intros H1 H2. rewrite sirreducible_comp. split7 ; triv.
+    rewrite sirreducible_ren. triv.
+Qed.
+
+(*********************************************************************************)
+(** *** [rename_aux] *)
+(*********************************************************************************)
+
+Equations rename_aux {k} (r : ren) (e : expr k) : expr k :=
+rename_aux R_id t := t ;
+rename_aux (R_cons i _) (E_tvar Q_zero) := tnat i ;
+rename_aux r t := E_ren r t.
+
+Lemma rename_aux_red {k} r (t : expr k) : 
+  E_ren r t =e=> rename_aux r t.
+Proof. funelim (rename_aux r t) ; simp red ; triv. Qed.
+#[local] Hint Rewrite <-@rename_aux_red : red.
+
+Lemma rename_aux_irreducible {k} r (t : expr k) :
+  rirreducible r -> eirreducible t -> 
+  (r <> R_id -> ~(is_rcons r /\ is_tvar_zero t) -> eirreducible (E_ren r t)) ->
+  eirreducible (rename_aux r t).
+Proof.
+intros H1 H2 H3. funelim (rename_aux r t) ; triv.
+all: try solve [ apply H3 ; triv ].
+rewrite rirreducible_cons in H1. now apply tnat_irreducible.
+Qed.
+
+(*********************************************************************************)
+(** *** [substitute_aux] *)
+(*********************************************************************************)
+
+(** Helper function for [rename] and [substitute] which takes care of trivial cases. *)
+Equations substitute_aux {k} (s : subst) (t : expr k) : expr k :=
+substitute_aux S_id t := t ;
+substitute_aux (S_cons t _) (E_tvar Q_zero) := t ;
+substitute_aux (S_ren r) t := E_ren r t ;
+substitute_aux s t := E_subst s t.
+
+Lemma substitute_aux_red {k} s (t : expr k) :
+  E_subst s t =e=> substitute_aux s t.
+Proof. funelim (substitute_aux s t) ; triv. Qed.
+#[local] Hint Rewrite <-@substitute_aux_red : red.
+
+Lemma substitute_aux_irreducible {k} s (t : expr k) :
+  eirreducible t -> sirreducible s -> 
+  match s with S_ren r => eirreducible (E_ren r t) | _ => True end ->
+  (s <> S_id -> ~(is_tvar_zero t /\ is_scons s) -> ~is_sren s -> eirreducible (E_subst s t)) ->
+  eirreducible (substitute_aux s t).
+Proof.
+intros H1 H2 H3 H4. funelim (substitute_aux s t) ; triv.
+all: try solve [ apply H4 ; triv ].
+now rewrite sirreducible_cons in H2.
+Qed.
+
+(*********************************************************************************)
+(** *** [rename] and [srcomp] *)
+(*********************************************************************************)
+
+Definition rup (r : ren) : ren := rcons Q_zero (rcomp r R_shift).
+
+(** Simplify [E_ren r t]. *)
+Equations rename {k} (r : ren) (t : expr k) : expr k by struct t :=
+rename r (E_tctor c al) := E_tctor c (rename r al) ;
+rename r E_al_nil := E_al_nil ;
+rename r (E_al_cons a al) := E_al_cons (rename r a) (rename r al) ;
+rename _ (E_abase b x) := E_abase b x ;
+rename r (E_aterm t) := E_aterm (rename r t) ;
+rename r (E_abind a) := E_abind (rename (rup r) a) ;
+rename r2 (E_ren r1 t) := rename_aux (rcomp r1 r2) t ;
+rename r (E_subst s t) := substitute_aux (srcomp s r) t ;
+rename r e := rename_aux r e 
+
+(** Simplify [S_comp s (S_ren r)]. *)
+with srcomp (s : subst) (r : ren) : subst by struct s :=
+srcomp S_id r := sren r ;
+srcomp (S_cons t s) r := scons (rename r t) (srcomp s r) ;
+srcomp (S_comp s1 s2) r := scomp_aux s1 (srcomp s2 r) ;
+srcomp s r := scomp_aux s (sren r). 
+
+Lemma rename_srcomp_red : 
+  (forall {k} r (t : expr k), E_ren r t =e=> rename r t) *
+  (forall s r, S_comp s (S_ren r) =s=> srcomp s r).
+Proof.
+apply rename_elim with 
+  (P := fun {k} r (t : expr k) res => E_ren r t =e=> res)
+  (P0 := fun s r res => S_comp s (S_ren r) =s=> res).
+all: intros.
+all: try solve [ triv | simp red ; triv | simp red ; now rewrite <-H ].
+- now rewrite <-H, <-H0.
+- rewrite <-H. unfold rup. simp red. triv.
+- simp red. rewrite <-H, <-H0. rewrite sred_cons_l. now rewrite ered_subst_sren.
+Qed.
+
+Lemma rename_red {k} r (t : expr k) :
+  E_ren r t =e=> rename r t. 
+Proof. now apply rename_srcomp_red. Qed.
+#[local] Hint Rewrite <-@rename_red : red.
+
+Lemma srcomp_red s r :
+  S_comp s (S_ren r) =s=> srcomp s r.
+Proof. now apply rename_srcomp_red. Qed.
+#[local] Hint Rewrite <-srcomp_red : red.
+
+Lemma rename_srcomp_irreducible :
+  (forall {k} r (t : expr k), rirreducible r -> eirreducible t -> eirreducible (rename r t)) *
+  (forall s r, sirreducible s -> rirreducible r -> sirreducible (srcomp s r)).
+Proof.
+apply rename_elim with 
+  (P := fun {k} r (t : expr k) res => rirreducible r -> eirreducible t -> eirreducible res)
+  (P0 := fun s r res => sirreducible s -> rirreducible r -> sirreducible res).
+all: intros ; triv.
+- rewrite eirreducible_tvar in H0. apply rename_aux_irreducible ; triv.
+  + now rewrite eirreducible_tvar.
+  + intros H1 H2. rewrite eirreducible_ren. split5 ; triv.
+    rewrite eirreducible_tvar. triv.
+- rewrite eirreducible_tctor in *. now apply H.
+- apply rename_aux_irreducible ; triv.
+  intros H1 H2. rewrite eirreducible_ren. split5 ; triv.
+- rewrite eirreducible_al_cons in *. split ; [apply H | apply H0] ; triv.
+- rewrite eirreducible_aterm in *. now apply H.
+- rewrite eirreducible_abind in *. apply H ; triv. unfold rup. 
+  apply rcons_irreducible ; triv. apply rapply_rcomp_irreducible ; triv.
+- rewrite eirreducible_ren in H0. apply rename_aux_irreducible ; triv.
+  + now apply rapply_rcomp_irreducible.
+  + intros H1 H2. rewrite eirreducible_ren. split5 ; triv.
+    now apply rapply_rcomp_irreducible.  
+- rewrite eirreducible_subst in H1. feed2 H ; triv.
+  apply substitute_aux_irreducible ; triv.
+  + destruct (srcomp s r) ; triv. rewrite sirreducible_ren in H. destruct r0 ; triv.
+    rewrite eirreducible_ren. triv.
+  + intros H4 H5 H6. rewrite eirreducible_subst. triv.
+- now apply sren_irreducible.
+- apply scomp_aux_irreducible ; triv. 
+  + now apply sren_irreducible.
+  + intros H1 H2. rewrite sirreducible_comp. split7 ; triv.
+    now apply sren_irreducible.
+- rewrite sirreducible_cons in H1. apply scons_irreducible.
+  + now apply H.
+  + now apply H0.
+- rewrite sirreducible_comp in H0. apply scomp_aux_irreducible ; triv.
+  + now apply H.
+  + intros H2 H3. rewrite sirreducible_comp. split7 ; triv.
+    now apply H.
+- rewrite sirreducible_ren in H. destruct r0 ; triv. apply scomp_aux_irreducible.
+  + now rewrite sirreducible_ren.
+  + now apply sren_irreducible.
+  + intros H1 H2. rewrite sirreducible_comp. split7 ; triv. 
+    * now rewrite sirreducible_ren.
+    * now apply sren_irreducible.
+- apply scomp_aux_irreducible ; triv.
+  + now apply sren_irreducible.
+  + intros H1 H2. rewrite sirreducible_comp. split7 ; triv.
+    now apply sren_irreducible.
+Qed. 
+
+(*********************************************************************************)
+(** *** [substitute] and [scomp] *)
+(*********************************************************************************)
+
+(** Lift a substitution through a binder. *)
+Definition sup (s : subst) : subst := scons (E_tvar Q_zero) (srcomp s R_shift).
+
+(** Apply an irreducible substitution to an irreducible expression. *)
+Equations substitute {k} (s : subst) (t : expr k) : expr k by struct t :=
+substitute s (E_tvar i) := sapply s i ;
+substitute s (E_tctor c al) := E_tctor c (substitute s al) ;
+substitute _ E_al_nil := E_al_nil ;
+substitute s (E_al_cons a al) := E_al_cons (substitute s a) (substitute s al) ;
+substitute _ (E_abase b x) := E_abase b x ;
+substitute s (E_aterm t) := E_aterm (substitute s t) ;
+substitute s (E_abind a) := E_abind (substitute (sup s) a) ;
+substitute s (E_ren r e) := substitute_aux (rscomp r s) e ;
+substitute s2 (E_subst s1 e) := substitute_aux (scomp s1 s2) e ;
+substitute s e := substitute_aux s e 
+
+(** Compose two irreducible substitutions. *)
+with scomp (s1 s2 : subst) : subst by struct s1 :=
+scomp S_id s := s ;
+scomp (S_cons t s1) s2 := scons (substitute s2 t) (scomp s1 s2) ;
+scomp (S_comp s1 s2) s3 := scomp_aux s1 (scomp s2 s3) ;
+scomp s1 s2 := scomp_aux s1 s2. 
+
+Lemma substitute_scomp_red : 
+  (forall {k} s (t : expr k), E_subst s t =e=> substitute s t) *
+  (forall s1 s2, S_comp s1 s2 =s=> scomp s1 s2).
+Proof.
+apply substitute_elim with
+  (P := fun {k} s (t : expr k) res => E_subst s t =e=> res)
+  (P0 := fun s1 s2 res => S_comp s1 s2 =s=> res).
+all: intros ; simp red ; triv.
+- now rewrite <-H.
+- now rewrite <-H, <-H0.
+- now rewrite <-H.
+- rewrite <-H. unfold sup. rewrite ered_subst_abind. now simp red.
+- now rewrite <-H.
+- now rewrite <-H, <-H0.
+- now rewrite <-H.
+Qed.
+
+Lemma substitute_red {k} s (t : expr k) :
+  E_subst s t =e=> substitute s t.
+Proof. now apply substitute_scomp_red. Qed.
+#[local] Hint Rewrite <-@substitute_red : red.
+
+Lemma scomp_red s1 s2 : S_comp s1 s2 =s=> scomp s1 s2.
+Proof. now apply substitute_scomp_red. Qed.
+#[local] Hint Rewrite <-scomp_red : red.
+
+Lemma substitute_scomp_irreducible : 
+  (forall {k} s (t : expr k), sirreducible s -> eirreducible t -> eirreducible (substitute s t)) *
+  (forall s1 s2, sirreducible s1 -> sirreducible s2 -> sirreducible (scomp s1 s2)).
+Proof.
+apply substitute_elim with   
+  (P := fun {k} s (t : expr k) res => sirreducible s -> eirreducible t -> eirreducible res)
+  (P0 := fun s1 s2 res => sirreducible s1 -> sirreducible s2 -> sirreducible res).
+all: intros ; triv.
+- apply sapply_rscomp_irreducible ; triv. rewrite eirreducible_tvar in H0.  
+  destruct H0. destruct i ; triv. all: exfalso ; triv.
+- rewrite eirreducible_tctor in *. now apply H.
+- apply substitute_aux_irreducible ; triv.
+  + destruct s ; triv. rewrite eirreducible_ren. rewrite sirreducible_ren in H.
+    destruct r ; triv.
+  + intros H1 H2 H3. rewrite eirreducible_subst. triv. 
+- rewrite eirreducible_al_cons in *. feed2 H ; triv. feed2 H0 ; triv.
+- rewrite eirreducible_aterm in *. now apply H.
+- rewrite eirreducible_abind in *. apply H ; triv. unfold sup.
+  apply scons_irreducible ; triv. apply rename_srcomp_irreducible ; triv.
+- rewrite eirreducible_ren in H0.
+  assert (H1 : sirreducible (rscomp r s)). { apply sapply_rscomp_irreducible ; triv. }
+  apply substitute_aux_irreducible ; triv.
+  + destruct (rscomp r s) ; triv. rewrite eirreducible_ren in *. rewrite sirreducible_ren in H1.
+    destruct r0 ; triv.
+  + intros H2 H3 H4. rewrite eirreducible_subst. split6 ; triv.  
+- rewrite eirreducible_subst in H1. feed2 H ; triv. apply substitute_aux_irreducible ; triv.
+  + destruct (scomp s1 s2) ; triv. rewrite sirreducible_ren in H. rewrite eirreducible_ren.
+    destruct r ; triv.
+  + intros H4 H5 H6. rewrite eirreducible_subst. triv.
+- apply scomp_aux_irreducible ; triv. intros H1 H2. rewrite sirreducible_comp. triv.
+- rewrite sirreducible_cons in *. feed2 H ; triv. feed2 H0 ; triv. 
+  apply scons_irreducible ; triv.
+- rewrite sirreducible_comp in H0. feed2 H ; triv. apply scomp_aux_irreducible ; triv.
+  intros H4 H5. rewrite sirreducible_comp. triv.
+- rewrite sirreducible_ren in H. destruct r ; triv. apply scomp_aux_irreducible ; triv.
+  + rewrite sirreducible_ren. triv.
+  + intros H1 H2. rewrite sirreducible_comp. split7 ; triv.
+    rewrite sirreducible_ren ; triv.
+- apply scomp_aux_irreducible ; triv. intros H1 H2. rewrite sirreducible_comp. triv.
+Qed.
+
+(*********************************************************************************)
+(** *** [esimp] and [ssimp] *)
+(*********************************************************************************)
+
+(** Simplify an expression. *)
+Equations esimp {k} (t : expr k) : expr k :=
+esimp (E_tvar i) := tnat (qsimp i) ;
+esimp (E_tctor c al) := E_tctor c (esimp al) ;
+esimp E_al_nil := E_al_nil ;
+esimp (E_al_cons a al) := E_al_cons (esimp a) (esimp al) ;
+esimp (E_abase b x) := E_abase b x ;
+esimp (E_aterm t) := E_aterm (esimp t) ;
+esimp (E_abind a) := E_abind (esimp a) ;
+esimp (E_ren r t) := rename (rsimp r) (esimp t) ;
+esimp (E_subst s t) := substitute (ssimp s) (esimp t) ;
+esimp (E_mvar m) := E_mvar m 
+
+(** Simplify a substitution. *)
+with ssimp (s : subst) : subst :=
+ssimp S_id := S_id ;
+ssimp S_shift := S_shift ;
+ssimp (S_cons t s) := scons (esimp t) (ssimp s) ;
+ssimp (S_comp s1 s2) := scomp (ssimp s1) (ssimp s2) ;
+ssimp (S_ren r) := sren (rsimp r) ;
+ssimp (S_mvar m) := S_mvar m.
+
+Lemma esimp_ssimp_red :
+  (forall {k} (t : expr k), t =e=> esimp t) *
+  (forall s, s =s=> ssimp s).
+Proof.
+apply esimp_elim with 
+  (P := fun _ t res => t =e=> res)
+  (P0 := fun s res => s =s=> res).
+all: intros ; simp red ; triv.
+all: solve [ now rewrite <-H | now rewrite <-H, <-H0 ]. 
+Qed.
+
+Lemma esimp_red {k} (t : expr k) : t =e=> esimp t.
+Proof. now apply esimp_ssimp_red. Qed.
+#[local] Hint Rewrite <-@esimp_red : red.
+
+Lemma ssimp_red s : s =s=> ssimp s.
+Proof. now apply esimp_ssimp_red. Qed.
+#[local] Hint Rewrite <-ssimp_red : red.
+
+Lemma esimp_ssimp_irreducible :
+  (forall {k} (t : expr k), eirreducible (esimp t)) *
+  (forall s, sirreducible (ssimp s)).
+Proof.
+apply esimp_elim with 
+  (P := fun _ _ res => eirreducible res) 
+  (P0 := fun _ res => sirreducible res).
+all: intros ; triv.
+- apply tnat_irreducible. apply qsimp_irreducible. 
+- now rewrite eirreducible_tctor.
+- now rewrite eirreducible_al_cons.
+- now rewrite eirreducible_aterm.
+- now rewrite eirreducible_abind.
+- apply rename_srcomp_irreducible ; triv. now apply rsimp_irreducible.
+- apply substitute_scomp_irreducible ; triv.
+- now apply scons_irreducible.
+- apply substitute_scomp_irreducible ; triv.
+- apply sren_irreducible. now apply rsimp_irreducible.
+Qed.
+
+Lemma esimp_irreducible {k} (t : expr k) : eirreducible (esimp t).
+Proof. now apply esimp_ssimp_irreducible. Qed.
+
+Lemma ssimp_irreducible s : sirreducible (ssimp s).
+Proof. now apply esimp_ssimp_irreducible. Qed.
+
+End WithSignature.
