theories/Prelude.v
@@ -20,7 +20,6 @@ Coercion is_true : bool >-> Sortclass.
 (** Add some power to [auto] and variants (such as [triv]). *)
 #[export] Hint Extern 5 => f_equal : core.
 #[export] Hint Extern 5 => subst : core.
-#[export] Hint Extern 10 => exfalso : core.
 
 (** Split n-ary conjunctions. *)
 Ltac split3 := split ; [|split].
